## 2023/11/22

> 作业：查咖啡环效应、“葡萄酒的眼泪”是什么

*将拉格朗日力学用于爱情，则 $L = T - V$ 中， $T$ 对应干劲，而 $S$ 表示气场。气场的来源则可能是财力、官阶……*

### 1. Features of classical mechanics 经典力学的特性

| Person | Year | Main Work | Space | Geometry |
| ------ | ---- | --------- | ----- | -------- |
| Newton | 1687 | *the Principia* <br> (《自然哲学的数学原理》) | Euclidean Space <br> (欧氏空间) | Euclidean Geometry <br> (欧氏几何) |
| Lagrange | 1788 | Analytical mechanics <br> (分析力学) | Configuration Space <br> (位形空间) | Riemannian geometry <br> (黎曼几何) |
| Hamilton | 1834 | Analytical mechanics <br> (分析力学) | Phase Space <br> (相空间) | Symplectic geometry <br> (辛几何) |

*拉格朗日把欧拉视为他的“学术导师”，故 $\displaystyle {\mathrm d \over \mathrm dt} {\partial L \over \partial \dot x}- {\partial L \over \partial x}=0$ 有欧拉-拉格朗日方程之名。*

### 2. Galilean transformation in Lagrangian mechanics 拉格朗日力学中的伽利略变换

#### (1) The principle of least action 最小作用量原理

1744, Maupertuis (莫培督) proposed **action (作用量, later known as Hamiltonian action 哈密顿作用量)**: $$S = \int L(q, \dot{q}, t) \mathrm{d} t.$$

In a mechanical system, we suppose that at instances $t_1$ and $t_2$, the position of coordinates are respectively $q^{(1)}$ and $q^{(2)}$. The condition is that the system shall move between these positions in a way that the integral $\displaystyle S = \int_{t_1}^{t_2} L(q, \dot{q}, t) \mathrm{d} t$ takes the least possible value.

This means that $\delta q(t_1) = \delta q(t_2) = 0$.

At such a place, we have $$\delta S = 0.$$

Let $$L' = L + \dfrac{\mathrm{d}f}{\mathrm{d}t}$$ where $f = f(q, t)$, and we get $$S' = \int_{t_1}^{t_2} \left[ L(q, \dot{q}, t) + \dfrac{\mathrm{d}f(q, t)}{\mathrm{d}t} \right] \mathrm{d}t = S + f(q, t) \Big|_{t_1}^{t_2}$$

#### (2) Galilean transformation 伽利略变换

In a Galilean transformation $\left\{ \begin{array}{l}
    \boldsymbol{r}' = \boldsymbol{r} - \boldsymbol{V}t \\
    t' = t
\end{array} \right.$ where we assume that the potential energy $U(q)$ is unchanged, we have $\boldsymbol{v}' = \boldsymbol{v} - \boldsymbol{V}$, and $$\begin{align*}
    L' = T' - U' & = {1 \over 2}m \boldsymbol{v}' \cdot \boldsymbol{v}' - U \\
    & = {1 \over 2}m \left( \boldsymbol{v} - \boldsymbol{V} \right) \cdot \left( \boldsymbol{v} - \boldsymbol{V} \right) - U \\
    & = {1 \over 2}m \boldsymbol{v} \cdot \boldsymbol{v} - m \boldsymbol{v} \cdot \boldsymbol{V} + {1 \over 2}m \boldsymbol{V} \cdot \boldsymbol{V} - U \\
    & = T - m \dfrac{\mathrm{d} \boldsymbol{r}}{\mathrm{d}t} \cdot \boldsymbol{V} + {1 \over 2} mV^2 - U \\
    & = L - m \dfrac{\mathrm{d}}{\mathrm{d}t} \left( \boldsymbol{r} \cdot \boldsymbol{V} - {1 \over 2}V^2 t \right).
\end{align*}$$

This means that under Galilean transformations, the Lagrangian $L$ stays equivalent.

### 3. Gauge Invariance 规范不变性 (考！)

#### (1) Basic forms of gauge transformation 规范场变换的基本形式

From the second equation of the Maxwell equations $$\nabla \cdot \boldsymbol B = 0,$$ we can see $B$ as the curl of a certain vector $\boldsymbol A$. We call this $\boldsymbol A$ **magnetic vector potential** (磁矢势), and $$\boldsymbol B  = \nabla \times \boldsymbol A.$$

Because the curl of the gradient of a certain scalar (标量梯度的旋度) is zero, we can add a scalar field $\psi$, and 

$$\boldsymbol A \mapsto \boldsymbol A + \nabla \psi \  (*)$$

$$\boldsymbol B  = \nabla \times (\boldsymbol A + \nabla \psi).$$

From $$\nabla \times \boldsymbol E = -{\partial \boldsymbol B \over \partial t}$$ and put the $\boldsymbol B$ in, we can get $$\nabla \times \boldsymbol E = - {\partial \over \partial t}(\nabla \times \boldsymbol A) = - \nabla \times {\partial \boldsymbol A \over \partial t}$$

$$\nabla \times (\boldsymbol E + {\partial \boldsymbol A \over \partial t}) = \boldsymbol 0.$$

From this we can see $\boldsymbol E + \dfrac{\partial \boldsymbol A }{ \partial t}$ as the negative of the gradient of a scalar field $\varphi$ (标量场 $\varphi$ 梯度的负), and $$\boldsymbol E = - \dfrac{\partial \boldsymbol A }{ \partial t} - \nabla \varphi.$$

When we put in the $\boldsymbol A$ shown by $(*)$, we can get:

$$
\begin{align*}
\boldsymbol E & = - \dfrac{\partial}{ \partial t}(\boldsymbol A + \nabla \psi) - \nabla \varphi \\[2ex]
& = - \dfrac{\partial \boldsymbol A }{ \partial t} - \nabla \left(\varphi + {\partial \psi \over \partial t}\right).
\end{align*}
$$

This shows that, when we make the transformation below (**the gauge transformation** 规范变换)

$$
\left\{
\begin{array} {l}
\boldsymbol A \mapsto \boldsymbol A + \nabla \psi \\[1ex]
\varphi \mapsto \varphi - \dfrac{\partial \psi}{\partial t}
\end{array}
\right.
$$

We can ensure that the fields $\boldsymbol B$ and $\boldsymbol E$ remain unchanged.

#### (2) Gauge invariance in magnetic fields 电磁场中的规范不变性

In a magnetic field with electric field (电场) $\boldsymbol{E}$ and electric potential (电势) $\varphi$ we have the electromagnetic force (电磁力) $$\begin{align*}
    \boldsymbol{F} & = q \left( \boldsymbol{E} + \boldsymbol{v} \times \boldsymbol{B} \right) \\
    & = q \left[ - \nabla \varphi - \dfrac{\partial \boldsymbol A }{\partial t} + \boldsymbol{v} \times \left( \nabla_{\boldsymbol{A}} \times \boldsymbol{A} \right) \right] \\
    & = q \left[ - \nabla \varphi - \dfrac{\partial \boldsymbol A }{\partial t} + \nabla_{\boldsymbol{A}} \left( \boldsymbol{v} \cdot \boldsymbol{A} \right) - \left( \boldsymbol{v} \cdot \nabla_{\boldsymbol{A}} \right) \boldsymbol{A} \right] \\
    & = q \left[ - \nabla \left( \varphi - \boldsymbol{v} \cdot \boldsymbol{A} \right) - \dfrac{\partial \boldsymbol A }{\partial t} - \left( \boldsymbol{v} \cdot \nabla_{\boldsymbol{A}} \right) \boldsymbol{A} \right] \\
    & = q \left( - \nabla U' - \dfrac{\mathrm{d} \boldsymbol{A}}{\mathrm{d}t} \right),
\end{align*}$$ where $\nabla_{\boldsymbol{A}}$ means the operator $\nabla$ operates exclusively on $\boldsymbol{A}$.

(Here you should note that $\displaystyle {\partial \over \partial t} + \boldsymbol{v} \cdot \nabla = \frac{\mathrm{d}}{\mathrm{d}t}$.)

So the Lagrangian in the original field $$L = {1 \over 2} mv^2 - q(\varphi - \boldsymbol{v} \cdot \boldsymbol{A})$$ and after the gauge transformation $$\begin{align*}
    L' & = {1 \over 2} m v^2 - q(\varphi' - \boldsymbol{v} \cdot \boldsymbol{A}') \\
    & = {1 \over 2} m v^2 - q \left[ \varphi - {\partial \psi \over \partial t} - \boldsymbol{v} \cdot \left( \boldsymbol{A} + \nabla \psi \right) \right] \\
    & = {1 \over 2} m v^2 - q(\varphi - \boldsymbol{v} \cdot \boldsymbol{A}) - q \left( {\partial \psi \over \partial t} + (\boldsymbol{v} \cdot \nabla) \psi \right) \\
    & = L - q \frac{\mathrm{d} \psi}{\mathrm{d}t} \\
    & = L - \frac{\mathrm{d}}{\mathrm{d}t} (q \psi).
\end{align*}$$

Because $- \dfrac{\mathrm{d}}{\mathrm{d}t} (q \psi)$ is a function of $q$ and $t$, we can see that after a gauge transformation, the Lagrangian stays equivalent to before. That is to say, after gauge transformations the principle of least action still holds, and we call this feature **gauge invariance (规范不变性)**.

### 4. Isochronic variation 等时变分

*译者注：isochronic variation这个翻译未经验证，不一定准确，仅供参考！*

The key information here is: $$\delta t = 0.$$

We can assume that $\mathrm{d}$ and $\partial$ can exchange themselves — that is, $$\delta \left( \dfrac{\mathrm{d}x}{\mathrm{d}t} \right) = \dfrac{\mathrm{d} (\delta x)}{\mathrm{d}t}.$$

Let $$\begin{align*} \delta \left( \dfrac{\mathrm{d}x}{\mathrm{d}t} \right) & = \dfrac{ \delta (\mathrm{d} x) \mathrm{d} t - \mathrm{d} x \delta (\mathrm{d} t)}{\mathrm{d} t^2} \\
    & = \dfrac{\mathrm{d} (\delta x) \mathrm{d} t}{\mathrm{d} t^2} - \dfrac{\mathrm{d} x \delta (\mathrm{d}t)}{\mathrm{d} t^2} \\
    & = \dfrac{\mathrm{d} (\delta x)}{\mathrm{d} t},
\end{align*}$$ we can see that $\delta (\mathrm{d}t) = \mathrm{d} (\delta t) = 0$.

$$\delta q(t_1) = \delta q(t_2) = 0$$

The Riemann metric tensor (黎曼度规张量) is $$\dfrac{\partial \boldsymbol{r}_\alpha}{\partial q_i} \cdot \dfrac{\partial \boldsymbol{r}_\alpha}{\partial q_j} = \mathbf{g}_{ij},$$ and in Riemann geometry we have $$\mathbf{a}_{ij} = \sum_{\alpha} m_\alpha \dfrac{\partial \boldsymbol{r}_\alpha}{\partial q_i} \cdot \dfrac{\partial \boldsymbol{r}_\alpha}{\partial q_j} = \sum_{\alpha} m_\alpha \mathbf{g}_{ij}.$$
