## 2023/11/15

### 1. Mechanical similarity 力学相对性

From *Mathematical Method in Classical Mechanics* by Vladimir Igorevich Arnold (Russian: Влади́мир И́горевич Арно́льд, 中文：弗拉基米尔·伊戈列维奇·阿诺尔德).

*上面这个人在19岁（1957年）时解决了希尔伯特第十三问题，名满天下！要向他学习！*

> 作业1：什么是希尔伯特第十三问题？是何时解决的？
>
>    答案：希尔伯特第十三问题是：$f^7 + x f^3 +y f^2 + zf + 1 = 0$ 这个方程式的七个解$f$，若表成$x, y, z$的函数，是否可以化成两个变量函数的组合 $f \circ g$。
>
>    1957年，阿诺尔德解决了这个问题，答案是“是”。

> 作业2：为什么所有动物跳的高度都是同一量级？

Assume that a potential energy in a system $U(\boldsymbol{r}_1, \boldsymbol{r}_2, \dots, \boldsymbol{r}_n)$ is a homogeneous function of degree $k$. This means that

$$U(\alpha \boldsymbol{r}_1, \alpha \boldsymbol{r}_2, \dots, \alpha \boldsymbol{r}_n) = \alpha^k U(\boldsymbol{r}_1, \boldsymbol{r}_2, \dots, \boldsymbol{r}_n).$$

Thus the Lagrangian (拉格朗日量) $L$ is 

$$L = T - U = \sum_{n} {1 \over 2} m {\mathrm{d} \boldsymbol{r}_i \over \mathrm{d} t} \cdot {\mathrm{d} \boldsymbol{r}_i \over \mathrm{d} t} - U(\boldsymbol{r}_1, \boldsymbol{r}_2, \dots, \boldsymbol{r}_n).$$

> 作业3：为什么拉格朗日量 $L = T - U$？

Let $\boldsymbol{r}_1' = \alpha \boldsymbol{r}_1$, $t' = \beta t$, and

$$L' = T' - U' = \left( {\alpha \over \beta} \right)^2 T - \alpha^k U.$$

To let the Euler–Lagrange equation $$\frac{\partial L}{\partial q} - \frac{\mathrm{d}}{\mathrm{d}t}\frac{\partial L}{\partial \dot q} = 0$$ still hold, we need $$\left( {\alpha \over \beta} \right)^2 = \alpha^k$$ or $${t' \over t} = \left( {l' \over l} \right)^{1 - k/2}.$$

Following this we can know some other physical quantities, for example:

$${E' \over E} = {U' \over U} = \alpha^k$$

$${\boldsymbol{v}' \over \boldsymbol{v}} = {l'/t' \over l/t} = {\alpha \over \beta} = \alpha^{k/2}$$

$${\boldsymbol{L}' \over \boldsymbol{L}} = {mv'l' \over mvl} = {\alpha^2 \over \beta} = \alpha^{1 + k/2}$$

Some applications of this include:

1. In the universal gravity field, $k = -1$, and $${t' \over t} = \left( {l' \over l} \right)^{3/2},$$ which is in accordance with **Kepler's Third Law (开普勒第三定律)**.

2. For a string, $k = 2$, and $${t' \over t} = \left( {l' \over l} \right)^{0} = 1,$$ which means that the period $T$ is independent of the amplitude of the string $A$.

> 作业4：
>
> 1. 质量不同势能相同的质点沿着相同轨道运动，它们的运动时间满足什么关系？
>
>    答案：$${t' \over t} = \sqrt{m' \over m}$$
>
> 2. 质点有相同的质量但势能相差一个常数因子，试求沿着相同轨道运动的时间之比？
>
>    答案：$${t' \over t} = \sqrt{U \over U'}$$

> 作业5：使用量纲分析多米诺骨牌倒下用时与相关物理量的关系

From Newton's second law of motion, we know that

$$\boldsymbol{F} = \dfrac{\mathrm{d} \boldsymbol{p}}{\mathrm{d}t}.$$

Under a potential field $U$, we have $$\boldsymbol{F} = - {\partial U \over \partial q}$$ and $$\boldsymbol{p} = {\partial T \over \partial \dot{q}},$$ and consequently, $$- {\partial U \over \partial q} = \dfrac{\mathrm{d}}{\mathrm{d}t} {\partial T \over \partial \dot{q}}.$$

Because $U = U(q_1, q_2, \dots, q_n)$ and $T = T(\dot{q}_1, \dot{q}_2, \dots, \dot{q}_n)$, we have $${\partial U \over \partial \dot{q}} = 0$$ and $${\partial T \over \partial q} = 0.$$

From these we can have $${\partial (T - U) \over \partial q} - \dfrac{\mathrm{d}}{\mathrm{d}t} {\partial (T - U) \over \partial \dot{q}} = 0,$$

$${\partial L \over \partial q} - \dfrac{\mathrm{d}}{\mathrm{d}t} {\partial L \over \partial \dot{q}} = 0,$$

### 2. Euler's equations in rigid body dynamics and the intermediate axis theorem 刚体运动的欧拉方程和中间轴定理

#### (1) Euler's equations in rigid body dynamics 刚体运动的欧拉方程

> 作业6：拉格朗日量 $L$ 为什么不写成 $\ddot q$ 的函数？

According to the angular momentum theorem (角动量定理), we have

$$\dfrac{\mathrm d \boldsymbol L}{\mathrm dt} = \boldsymbol M,$$

where $\boldsymbol M$ is the external torque (外力矩) and $\boldsymbol L = \mathbf I \boldsymbol \omega$. 

According to the transport theorem, 

$$\dfrac{\mathrm d \boldsymbol L}{\mathrm dt} = \left[ \dfrac{\mathrm d (\mathbf I \boldsymbol \omega)}{\mathrm dt}\right]_r + \boldsymbol \omega \times (\mathbf I \boldsymbol \omega) = \boldsymbol M$$

Because $\mathbf I$ is a constant, we have

$$
\mathbf I \left( \dfrac{\mathrm d \boldsymbol \omega}{\mathrm dt} \right)_r + 
\begin{vmatrix}
\hat i & \hat j & \hat k \\
\omega_1 & \omega_2 & \omega_3 \\
\mathrm I_{11} \omega_1 & \mathrm I_{22} \omega_2 & \mathrm I_{33} \omega_3 \\
\end{vmatrix} =
\begin{pmatrix}
M_1 \\ M_2 \\ M_3
\end{pmatrix}
$$

In orthogonal principal axes of inertia coordinates the equations become

$$
\left\{
\begin{align*}
\mathrm I_{11} \dfrac{\mathrm d \boldsymbol \omega_1}{\mathrm dt} + (\mathrm I_{33} - \mathrm I_{22}) \omega_2 \omega_3 & = M_1 \\[2ex]
\mathrm I_{22} \dfrac{\mathrm d \boldsymbol \omega_2}{\mathrm dt} + (\mathrm I_{11} - \mathrm I_{33}) \omega_1 \omega_3 & = M_2 \\[2ex]
\mathrm I_{33} \dfrac{\mathrm d \boldsymbol \omega_3}{\mathrm dt} + (\mathrm I_{22} - \mathrm I_{11}) \omega_1 \omega_2 & = M_3
\end{align*}
\right.
$$

#### (2) Intermediate axis theorem 中间轴定理

> 作业7：查一下礼炮七号发生的事故

*酒泉卫星发射中心：向航天强国奋力迈进*

The intermediate axis theorem is also called the tennis racket theorem (网球拍定理) or Dzhanibekov effect (贾尼别科夫效应). Vladimir Aleksandrovich Dzhanibekov (Russian: Владимир Александрович Джанибеков, 中文：弗拉基米尔·亚历山德罗维奇·贾尼别科夫) noticed a logical consequence of this theorem in space in 1985.

Now we assume that, for a rigid body, $\mathrm I_{11} > \mathrm I_{22} > \mathrm I_{33}$, and:

- Case 1: rotation around $\mathrm I_{11}$

    Here we assume that $\omega_1 = \Omega$, and $\omega_2, \omega_3 \ll \Omega$.

    $$
    \left\{
    \begin{align*}
    \mathrm I_{11} \dfrac{\mathrm d \boldsymbol \omega_1}{\mathrm dt} & = (\mathrm I_{22} - \mathrm I_{33}) \omega_2 \omega_3 \approx 0 \\[2ex]
    \mathrm I_{22} \dfrac{\mathrm d \boldsymbol \omega_2}{\mathrm dt} & = (\mathrm I_{33} - \mathrm I_{11}) \Omega \omega_3 \\[2ex]
    \mathrm I_{33} \dfrac{\mathrm d \boldsymbol \omega_3}{\mathrm dt} & = (\mathrm I_{11} - \mathrm I_{22}) \Omega \omega_2
    \end{align*}
    \right.
    $$

    Take the time derivatives of these equations, and we get

    $$
    \left\{
    \begin{align*}
    \mathrm I_{11} \dfrac{\mathrm d^2 \boldsymbol \omega_1}{\mathrm dt^2} & = 0 \\[2ex]
    \mathrm I_{22} \dfrac{\mathrm d^2 \boldsymbol \omega_2}{\mathrm dt^2} & = (\mathrm I_{33} - \mathrm I_{11}) \Omega \dfrac{\mathrm d \boldsymbol \omega_3}{\mathrm dt} = \dfrac{(\mathrm I_{33} - \mathrm I_{11})(\mathrm I_{11} - \mathrm I_{22})}{\mathrm I_{33}} \Omega^2 \omega_2 \\[2ex]
    \mathrm I_{33} \dfrac{\mathrm d^2 \boldsymbol \omega_3}{\mathrm dt^2} & = (\mathrm I_{11} - \mathrm I_{22}) \Omega \dfrac{\mathrm d \boldsymbol \omega_2}{\mathrm dt} = \dfrac{(\mathrm I_{33} - \mathrm I_{11})(\mathrm I_{11} - \mathrm I_{22})}{\mathrm I_{33}} \Omega^2 \omega_3
    \end{align*}
    \right.
    $$

    Here, we have ($\omega_3$ is similar to this)

    $$\ddot{\omega}_2 + \dfrac{(\mathrm I_{11} - \mathrm I_{33})(\mathrm I_{11} - \mathrm I_{22})}{\mathrm I_{22} \mathrm I_{33}} \Omega^2 \omega_2 = 0.$$

    Let $\dfrac{(\mathrm I_{11} - \mathrm I_{33})(\mathrm I_{11} - \mathrm I_{22})}{\mathrm I_{22} \mathrm I_{33}}  \Omega^2= \alpha_2$.

    Because $\alpha_2 > 0$, the general solution is

    $$\omega_2 = C_1 \sin \left( \sqrt{\alpha_2}t \right) + C_2 \cos \left( \sqrt{\alpha_2}t \right).$$

    This is a periodic, bounded function (周期性有界函数), which means that the rotation of directions $2$ and $3$ can be kept within a certain range.

- Case 2: rotation around $\mathrm I_{22}$

    Here we assume that $\omega_2 = \Omega$, and $\omega_1, \omega_3 \ll \Omega$.

    Similar to Case 1, we know that

    $$\ddot{\omega}_1 = \dfrac{(\mathrm I_{11} - \mathrm I_{22})(\mathrm I_{22} - \mathrm I_{33})}{\mathrm I_{11} \mathrm I_{33}} \Omega^2 \omega_1.$$

    Let $\dfrac{(\mathrm I_{11} - \mathrm I_{22})(\mathrm I_{22} - \mathrm I_{33})}{\mathrm I_{11} \mathrm I_{33}} \Omega^2 = \alpha_1$.

    Because $\alpha_1 > 0$, the general solution is

    $$\omega_1 = C_1 \exp \left( \sqrt{\alpha_1} t \right) + C_2 \exp \left( - \sqrt{\alpha_1} t \right)$$

    This is not a periodic, bounded function, which means that the rotation of direction $1$ can be kept within a certain range.