## 2023/11/27

### 1. Metric tensors 度规张量

*Feynman去做出租车，他不知道应该去哪个校区，于是他跟司机说：“去那个昨天有很多人去的地方，他们嘴上都说着什么 $\mu\nu$ 之类的东西”*

#### (1) Definition 定义

Define $$\mathbf{g} = g_{\mu\nu} \boldsymbol{e}^{\mu} \otimes \boldsymbol{e}^{\nu} = \frac{\partial \boldsymbol{r}}{\partial x_\mu} \cdot \frac{\partial \boldsymbol{r}}{\partial x_\nu} \boldsymbol{e}^{\mu} \otimes \boldsymbol{e}^{\nu}.$$

#### (2) Examples 例子

- Lorentzian metrics from relativity 相对论的洛伦兹度量

    In this case, the space-time interval can be written as $$\mathrm{d} s^2 = c^2 \mathrm{d}t^2 - \mathrm{d} x^2 - \mathrm{d} y^2 - \mathrm{d} z^2 = g_{\mu\nu} \mathrm{d}x^{\mu} \mathrm{d}x^{\nu},$$ where $\mathrm{d} s^2$ stands for $(\mathrm{d} s)^2$.

    From this we can see $$\mathbf{g} = \begin{pmatrix}
        1 & 0 & 0 & 0 \\
        0 & -1 & 0 & 0 \\
        0 & 0 & -1 & 0 \\
        0 & 0 & 0 & -1
    \end{pmatrix}.$$

    Also from this we can have $$\begin{align*} \mathrm{d} s^2 & = c^2 \mathrm{d}t^2 \left[ 1 - \frac{1}{c^2} \left( \frac{\mathrm{d}x}{\mathrm{d}t} \right)^2 - \frac{1}{c^2} \left( \frac{\mathrm{d}y}{\mathrm{d}t} \right)^2 - \frac{1}{c^2} \left( \frac{\mathrm{d}z}{\mathrm{d}t} \right)^2 \right] \\
        & = c^2 \mathrm{d}t^2 \left( 1 - {v^2 \over c^2} \right) \\
        & = c^2 \mathrm{d} \tau^2,
    \end{align*}$$ where $\tau$ is the **proper time (固有时)**, and $$\frac{\mathrm{d}t}{\mathrm{d} \tau} = \gamma = \frac{1}{\sqrt{1 - \dfrac{v^2}{c^2}}}.$$

- Cartesian coordinates 笛卡尔坐标系

    In this situation we have $\boldsymbol{r} = (x, y, z)$, and thus we have $$\frac{\partial \boldsymbol{r}}{\partial x} = (1, 0, 0)$$ $$\frac{\partial \boldsymbol{r}}{\partial y} = (0, 1, 0)$$ $$\frac{\partial \boldsymbol{r}}{\partial z} = (0, 0, 1).$$

    From this we know $$g_{xx} = g_{yy} = g_{zz} = 1, $$ and $$g_{xy} = g_{yx} = g_{xz} = g_{zx} = g_{yz} = g_{yz} =0.$$

    $$\mathbf{g} = \begin{pmatrix}
        1 & 0 & 0 \\
        0 & 1 & 0 \\
        0 & 0 & 1
    \end{pmatrix}.$$

- Cylindrical coordinates 柱坐标

    In this situation we have $\boldsymbol{r} = (r \cos \theta, r \sin \theta, z)$, or $$\mathrm{d} s^2 = \mathrm{d}r^2 + r^2 \mathrm{d} \theta^2 + \mathrm{d} z^2 = g_{\mu\nu} \mathrm{d}x^{\mu} \mathrm{d}x^{\nu}.$$

    Thus, we have $$\frac{\partial \boldsymbol{r}}{\partial r} = (\cos \theta, \sin \theta, 0)$$ $$\frac{\partial \boldsymbol{r}}{\partial \theta} = (-r \sin \theta, r \cos \theta, 0)$$ $$\frac{\partial \boldsymbol{r}}{\partial z} = (0, 0, 1).$$

    From this we know $$g_{rr} = \cos^2 \theta + \sin^2 \theta = 1,$$ $$g_{\theta \theta} = (-r \sin \theta)^2 + (r \cos \theta)^2 = r^2,$$ $$g_{zz} = 1.$$

    $$\mathbf{g} = \begin{pmatrix}
        1 & 0 & 0 \\
        0 & r^2 & 0 \\
        0 & 0 & 1
    \end{pmatrix}.$$

    
### 2. Tensor form of kinetic energy in Lagrangian systems

Suppose we have $N$ particles in the system and the kinetic energy $$T = \sum_{i = 1}^{N} {1 \over 2} m_i \boldsymbol{v}_i \cdot \boldsymbol{v}_i.$$

Usually we have the position of a particle $\boldsymbol{r}_i = \boldsymbol{r}_i(q_1, q_2, \dots, q_n; t)$. Take the total derivative (全微分) of $\boldsymbol{r}_i$ and we have $$\boldsymbol{v}_i = {\mathrm{d} \boldsymbol{r}_i \over \mathrm{d}t} = {\partial \boldsymbol{r}_i \over \partial t} + \sum_{\alpha = 1}^{n} {\partial \boldsymbol{r}_i \over \partial q_\alpha} {\mathrm{d} q_\alpha \over \mathrm{d}t}.$$

When the positions $\boldsymbol{r}_i$ doesn't explicitly contain time $t$, we have $${\partial \boldsymbol{r}_i \over \partial t} = 0$$ and $$\boldsymbol{v}_i =  \sum_{\alpha = 1}^{n} {\partial \boldsymbol{r}_i \over \partial q_\alpha} {\mathrm{d} q_\alpha \over \mathrm{d}t}.$$

Thus $$\begin{align*}
    T & = \sum_{i = 1}^{N} {1 \over 2} m_i \left( \sum_{\alpha = 1}^{n} {\partial \boldsymbol{r}_i \over \partial q_\alpha} {\mathrm{d} q_\alpha \over \mathrm{d}t} \right) \cdot \left( \sum_{\beta = 1}^{n} {\partial \boldsymbol{r}_i \over \partial q_\beta} {\mathrm{d} q_\beta \over \mathrm{d}t} \right) \\
    & = {1 \over 2} \sum_{\alpha, \beta = 1}^{n} \sum_{i = 1}^{N} m_i {\partial \boldsymbol{r}_i \over \partial q_\alpha} {\partial \boldsymbol{r}_i \over \partial q_\beta} {\mathrm{d} q_\alpha \over \mathrm{d}t} {\mathrm{d} q_\beta \over \mathrm{d}t} \\
    & = {1 \over 2} \sum_{\alpha, \beta = 1}^{n} a_{\alpha\beta} \dot{q}_\alpha \dot{q}_\beta \\
    & = {1 \over 2} \sum_{\alpha, \beta = 1}^{n} \dot{\mathbf{q}}_\alpha^{T} \cdot a_{\alpha \beta} \cdot \dot{\mathbf{q}}_\beta.
\end{align*}$$

### 3. Rayleigh dissipation function 瑞利耗散函数

Suppose we have $f = - \mu \dot{x}$, and we define the Rayleigh dissipation function $$R = {1 \over 2} \mu \dot{x}^2 = {1 \over 2} |f| \dot{x}.$$

When $R$ is added to the Euler-Lagrange equation, we acquire $${\mathrm{d} \over \mathrm{d}t} {\partial L \over \partial \dot q_\alpha} - {\partial L \over \partial q_\alpha} = - {\partial R \over \partial \dot q_\alpha}.$$


Also, in tensor form, we can have $$R = {1 \over 2} \boldsymbol{q}^T \cdot \mathbf{\mu} \cdot \boldsymbol{q}.$$
