## 2023/10/23

> 作业：黑洞熵是什么

*任正非：华为的自我批判性*

### 1. Something about Levi-Civita symbols and matrices

Consider a 3 by 3 matrix ($3 \times 3$ 矩阵) $\mathbf A$:

$$
\mathbf A=
\begin{bmatrix}
a_{11} & a_{12} & a_{13} \\
a_{21} & a_{22} & a_{23} \\
a_{31} & a_{32} & a_{33} \\
\end{bmatrix}
$$

$$
\begin{align*}
\det (\mathbf A) & =
\begin{vmatrix}
a_{11} & a_{12} & a_{13} \\
a_{21} & a_{22} & a_{23} \\
a_{31} & a_{32} & a_{33} \\
\end{vmatrix} \\
& = \varepsilon_{\alpha \beta \gamma} a_{1 \alpha} a_{2 \beta} a_{3 \gamma} = \varepsilon_{\alpha \beta \gamma} a_{2 \alpha} a_{3 \beta} a_{1 \gamma} = \varepsilon_{\alpha \beta \gamma} a_{3 \alpha} a_{1 \beta} a_{2 \gamma} \\ 
& = - \varepsilon_{\alpha \beta \gamma} a_{3 \alpha} a_{2 \beta} a_{1 \gamma} = - \varepsilon_{\alpha \beta \gamma} a_{1 \alpha} a_{3 \beta} a_{2 \gamma} = - \varepsilon_{\alpha \beta \gamma} a_{2 \alpha} a_{1 \beta} a_{3 \gamma} \\ 
\end{align*}
$$

Consider $(i, j, k)$  taking the following values, and $\varepsilon_{ijk} \varepsilon_{\alpha \beta \gamma} a_{i \alpha} a_{j \beta} a_{k \gamma}$:

$$
\begin{align*}
\text{even} &
\left\{
\begin{align*}
(1, 2, 3) & \ \ \ & \varepsilon_{123} \varepsilon_{\alpha \beta \gamma} a_{1 \alpha} a_{2 \beta} a_{3 \gamma} & = \det (\mathbf A) \\
(2, 3, 1) & \ \ \ & \varepsilon_{231} \varepsilon_{\alpha \beta \gamma} a_{2 \alpha} a_{3 \beta} a_{1 \gamma} & = \det (\mathbf A) \\
(3, 1, 2) & \ \ \ & \varepsilon_{312} \varepsilon_{\alpha \beta \gamma} a_{3 \alpha} a_{1 \beta} a_{2 \gamma} & = \det (\mathbf A) \\
\end{align*}
\right.
\\
\text{odd} &
\left\{
\begin{align*}
(3, 2, 1) & \ \ \ & \varepsilon_{321} \varepsilon_{\alpha \beta \gamma} a_{3 \alpha} a_{2 \beta} a_{1 \gamma} & = - \det (\mathbf A) \\
(2, 1, 3) & \ \ \ & \varepsilon_{213} \varepsilon_{\alpha \beta \gamma} a_{2 \alpha} a_{1 \beta} a_{3 \gamma} & = - \det (\mathbf A) \\
(1, 3, 2) & \ \ \ & \varepsilon_{132} \varepsilon_{\alpha \beta \gamma} a_{1 \alpha} a_{3 \beta} a_{2 \gamma} & = - \det (\mathbf A) \\
\end{align*}
\right.
\end{align*}
$$

Therefore, 

$$
\det (\mathbf A) = {1 \over 6} \varepsilon_{ijk} \varepsilon_{\alpha \beta \gamma} a_{i \alpha} a_{j \beta} a_{k \gamma}.
$$

### 2. Deduction of electromagnetic wave equations 电磁波方程推导

In vacuum (真空), $\rho = 0$ and $\vec j = \rho \vec v_d = \vec 0$, and Maxwell's equations degenerate into the following form:

$$
\left \{
\begin{array}{l} 
\overrightarrow \nabla \cdot \overrightarrow E = 0\\[2ex]
\overrightarrow \nabla \cdot \overrightarrow B = 0 \\[2ex]
\overrightarrow \nabla \times \overrightarrow E = -\dfrac{\partial B}{\partial t} \ (*)\\[2ex]
\overrightarrow \nabla \times \overrightarrow B = \mu_0 \varepsilon_0 \dfrac{\partial \overrightarrow E}{ \partial t} = \dfrac{1}{c^2} \dfrac{\partial \overrightarrow E}{ \partial t} \\
\end{array} 
\right.
$$

Get the curl of the left and right sides of $(*).$

Left-hand side:

$$
\begin {align*}
\overrightarrow \nabla \times (\overrightarrow \nabla \times \overrightarrow E) & = \overrightarrow \nabla \times \left({\partial E_j \over \partial x_i} \varepsilon_{ijk} \vec e_k \right) \\[2ex]
& = \left({\partial \over \partial x_\ell} \vec e_\ell \right) \times \left({\partial E_j \over \partial x_i} \varepsilon_{ijk} \vec e_k \right) \\[2ex]
& = {\partial^2 E_j \over \partial x_i \partial x_\ell} \varepsilon_{ijk} \varepsilon_{\ell k m} \vec e_m \\[2ex]
& = {\partial^2 E_j \over \partial x_i \partial x_\ell} \varepsilon_{ijk} \varepsilon_{m \ell k} \vec e_m \\[2ex]
& = {\partial^2 E_j \over \partial x_i \partial x_\ell} (\delta_{im}\delta_{j \ell} - \delta_{i \ell}\delta_{jm}) \vec e_m \\[2ex]
& = {\partial^2 E_j \over \partial x_i \partial x_j} \vec e_i - {\partial^2 E_j \over \partial x_i^2} \vec e_j \\[2ex]
& = \vec e_i {\partial \over \partial x_i}\left({\partial E_j \over \partial x_j}\right) - {\partial^2 \over \partial x_i^2} E_j \vec e_j \\[2ex]
& = \overrightarrow \nabla (\overrightarrow \nabla \cdot  \overrightarrow E) - \nabla^2 \overrightarrow E \\
& = - \nabla^2 \overrightarrow E
\end {align*}
$$

Right-hand side:

$$
\begin {align*}
\overrightarrow \nabla \times \left(-\dfrac{\partial B}{\partial t} \right) & = -\dfrac{\partial}{\partial t} \left( \overrightarrow \nabla \times \overrightarrow B \right) \\[2ex]
& = -\dfrac{\partial}{\partial t} \left(\dfrac{1}{c^2} \dfrac{\partial \overrightarrow E}{\partial t}\right) \\[2ex]
& = - \dfrac{1}{c^2} \dfrac{\partial^2 \overrightarrow E}{\partial t^2}
\end {align*}
$$

Consequently we have

$$ - \nabla^2 \overrightarrow E = - \dfrac{1}{c^2} \dfrac{\partial^2 \overrightarrow E}{\partial t^2}$$

$$\left(\dfrac{1}{c^2} \dfrac{\partial^2}{\partial t^2}- \nabla^2 \right) \overrightarrow E = \Box \overrightarrow E = \vec 0.$$

(This is a `2nd order partial differential equation 二阶偏微分方程`.)

Similarly we have:

Left-hand side:

$$
\begin {align*}
\overrightarrow \nabla \times (\overrightarrow \nabla \times \overrightarrow B) & = \overrightarrow \nabla \times \left({\partial E_j \over \partial x_i} \varepsilon_{ijk} \vec e_k \right) \\[2ex]
& = \overrightarrow \nabla (\overrightarrow \nabla \cdot  \overrightarrow B) - \nabla^2 \overrightarrow B \\
& = - \nabla^2 \overrightarrow B
\end {align*}
$$

Right-hand side:

$$
\begin {align*}
\overrightarrow \nabla \times \left(-\dfrac{\partial B}{\partial t} \right) & = \overrightarrow \nabla \times \left(\dfrac{1}{c^2} \dfrac{\partial \overrightarrow E}{\partial t}\right) \\
& = \dfrac{1}{c^2} \dfrac{\partial}{\partial t} (\overrightarrow \nabla \times \overrightarrow E) \\[2ex]
& = - \dfrac{1}{c^2} \dfrac{\partial^2 \overrightarrow B}{\partial t^2}
\end {align*}
$$

$$\left(\dfrac{1}{c^2} \dfrac{\partial^2}{\partial t^2}- \nabla^2 \right) \overrightarrow B = \Box \overrightarrow B = \vec 0.$$

Electromagnetic wave equations:

$$
\left\{
\begin{align*}
\left(\dfrac{1}{c^2} \dfrac{\partial^2}{\partial t^2}- \nabla^2 \right) \overrightarrow E = \vec 0 \\[2ex]
\left(\dfrac{1}{c^2} \dfrac{\partial^2}{\partial t^2}- \nabla^2 \right) \overrightarrow B = \vec 0
\end{align*}
\right.
$$

*考试晕倒：国科大优秀传统*

### 3. A second proof of some conclusions 一些结论的第二种证明 

#### (1) The curl of the gradient of any scalar field is always the zero vector field 梯度无旋

$$
\begin{align*}
\overrightarrow \nabla \times \left(\overrightarrow \nabla \varphi \right) & = \overrightarrow \nabla \times \left({\partial \varphi \over \partial x_i} \vec e_i \right) \\
& = {\partial \over \partial x_j} {\partial \varphi \over \partial x_i} \varepsilon_{jik} \vec e_k \\
& \overset{\text{interchange} \ i \ \mathrm{\&} \ j }{=\!=\!=\!=\!=\!=\!=\!=\!=\!=} {\partial \over \partial x_i} {\partial \varphi \over \partial x_j} \varepsilon_{ijk} \vec e_k \\
& \overset{\varphi \ 二阶光滑(二阶连续可导)}{=\!=\!=\!=\!=\!=\!=\!=\!=\!=\!=\!=\!=\!=\!=} {1 \over 2} \left({\partial^2 \varphi \over \partial x_i \partial x_j} \varepsilon_{jik} + {\partial^2 \varphi \over \partial x_i \partial x_j} \varepsilon_{ijk} \right) \vec e_k \\
& = \vec 0
\end{align*}
$$

#### (2) The divergence of the curl of any vector field is equal to zero 旋度无散

$$
\begin{align*}
\overrightarrow \nabla \cdot \left(\overrightarrow \nabla \times \overrightarrow A \right) & = \overrightarrow \nabla \cdot \left({\partial A_j \over \partial x_i} \varepsilon_{ijk} \vec e_k \right) \\
& = {\partial \over \partial x_\ell} {\partial A_j \over \partial x_i} \varepsilon_{ijk} \vec e_k \cdot \vec e_\ell \\
& \overset{\varphi 二阶光滑(二阶连续可导)}{=\!=\!=\!=\!=\!=\!=\!=\!=\!=\!=\!=\!=\!=} {1 \over 2} \left({\partial^2 \varphi \over \partial x_i \partial x_j} \varepsilon_{jik} + {\partial^2 \varphi \over \partial x_i \partial x_j} \varepsilon_{ijk} \right) \vec e_k \\
& = \vec 0
\end{align*}
$$

### 4. Vortices and vorticity 涡旋和涡量

*(译者注：vortex的复数形式为vortices)*

Vorticity is defined as the curl of the velocity of the field (速度场的旋度) $\overrightarrow \nabla \times \vec v$.

$$
\begin{align*}
\left(\overrightarrow \nabla \times \vec v \right) \times \vec v
& = \left({\partial v_j \over \partial x_i} \varepsilon_{ijk} \vec e_k \right) \times \left(v_\ell \vec e_\ell \right) \\
& = v_\ell {\partial v_j \over \partial x_i} \varepsilon_{ijk} \varepsilon_{\ell mk} \vec e_m \\
& = v_\ell {\partial v_j \over \partial x_i} (\delta_{i \ell}\delta_{jm} - \delta_{im}\delta_{j \ell}) \vec e_m \\
& = v_i {\partial v_j \over \partial x_i} \vec e_j - v_j {\partial v_j \over \partial x_i} \vec e_i \\
& = \left(v_i {\partial \over \partial x_i}\right) v_j \vec e_j - v_j {\partial v_j \over \partial x_i} \vec e_i \\
& = \left(\vec v \cdot \overrightarrow \nabla \right) \vec v - \overrightarrow \nabla \left( {1 \over 2} \vec v \cdot \vec v \right) \\
& = \left(\vec v \cdot \overrightarrow \nabla \right) \vec v - \overrightarrow \nabla \left( {1 \over 2} v^2 \right) \\
\end{align*}
$$

The material derivative (物质导数) of $\vec v$ is shown as follows:

$$\vec a = {\mathrm D \vec v \over \mathrm Dt} \equiv {\partial \vec v \over \partial t} + \left(\vec v \cdot \overrightarrow \nabla \right) \vec v = {\partial \vec v \over \partial t} + \left(\overrightarrow \nabla \times \vec v \right) \times \vec v + \overrightarrow \nabla \left( {1 \over 2} v^2 \right)$$

Consequently, the Navier-Stokes equations can be written as 

$$ {\partial \vec v \over \partial t} + \left(\overrightarrow \nabla \times \vec v \right) \times \vec v + \overrightarrow \nabla \left( {1 \over 2} v^2 \right) = -{1 \over \rho} \overrightarrow \nabla p + \mu \nabla^2 \vec v + \vec g,$$

where $\vec g = - \overrightarrow \nabla (gh).$
